{
 "cells": [
  {
   "cell_type": "markdown",
   "id": "86ab4a3c",
   "metadata": {},
   "source": [
    "# AEROSP 423 Computational Methods: Homework 1\n",
    "Jason Chen\n",
    "\n",
    "## Problem 1\n",
    "$$\n",
    "\\quad \\text{state:} \\quad \\mathbf{u} = \\begin{bmatrix} E \\\\ f_x/c^2 \\\\ f_y/c^2 \\end{bmatrix}, \\quad \\text{flux:} \\quad \\mathbf{F} = \\begin{bmatrix} f_x n_x + f_y n_y \\\\ \\frac{1}{3} E n_x \\\\ \\frac{1}{3} E n_y \\end{bmatrix}\n",
    "$$\n",
    "### Part (a)\n",
    "Calculate the flux Jacobian matrix.\n",
    "\n",
    "Generally speaking, the Jacobian matrix is:\n",
    "$$\n",
    "\\mathbf{A} = \\frac{\\partial \\mathbf{F}}{\\partial \\mathbf{u}} = \\begin{bmatrix} \\frac{\\partial F_1}{\\partial u_1} & \\frac{\\partial F_1}{\\partial u_2} & \\frac{\\partial F_1}{\\partial u_3} \\\\ \\frac{\\partial F_2}{\\partial u_1} & \\frac{\\partial F_2}{\\partial u_2} & \\frac{\\partial F_2}{\\partial u_3} \\\\ \\frac{\\partial F_3}{\\partial u_1} & \\frac{\\partial F_3}{\\partial u_2} & \\frac{\\partial F_3}{\\partial u_3} \\end{bmatrix}\n",
    "$$\n",
    "However, we need to write each component of the flux in terms of the state variables, e.g. $u_1$. So the flux matrix becomes:\n",
    "$$\n",
    "\\mathbf{F} = \\begin{bmatrix} c^2(u_2 n_x + u_3 n_y) \\\\ \\frac{1}{3} u_1 n_x \\\\ \\frac{1}{3} u_1 n_y \\end{bmatrix}\n",
    "$$\n",
    "So the Jacobian:\n",
    "$$\n",
    "\\mathbf{A} = \\begin{bmatrix} 0 & c^2 n_x & c^2 n_y \\\\ \\frac{1}{3}n_x & 0 & 0 \\\\ \\frac{1}{3}n_y & 0 & 0 \\end{bmatrix}\n",
    "$$\n"
   ]
  },
  {
   "cell_type": "markdown",
   "id": "089e99a6",
   "metadata": {},
   "source": [
    "### Part (b)\n",
    "Compute the eigenvalues and right eigenvectors of $\\mathbf{A}$.\n",
    "\n",
    "We will use the eigenvalue characteristic equation:\n",
    "$$\n",
    "\\mathbf{det}(A-\\lambda I ) = 0\n",
    "$$\n",
    "$$\n",
    "\\begin{vmatrix} -\\lambda & c^2 n_x & c^2 n_y \\\\ \\frac{1}{3}n_x & -\\lambda & 0 \\\\ \\frac{1}{3}n_y & 0 & -\\lambda \\end{vmatrix} = 0\n",
    "$$\n",
    "$$\n",
    "= -\\lambda(\\lambda^2) - c^2 n_x \\left( -\\lambda \\frac{1}{3}n_x \\right) + c^2 n_y \\left( \\lambda\\frac{1}{3} n_y \\right)\n",
    "$$\n",
    "$$\n",
    "= -\\lambda^3 + \\lambda\\frac{c^2}{3}(n_x^2 + n_y^2)\n",
    "$$"
   ]
  },
  {
   "cell_type": "markdown",
   "id": "8e3798e0",
   "metadata": {},
   "source": [
    "Since $\\vec{n}$ is a normal vector, the term $(n_x^2 + n_y^2)$ equals 1. So the characteristic equation becomes:\n",
    "$$\n",
    "\\lambda \\left( -\\lambda^2 + \\frac{c^2}{3}\\right) = 0\n",
    "$$\n",
    "Eigenvalues:\n",
    "$$\n",
    "\\lambda_1 = 0, \\quad \\lambda_2 = \\frac{c}{\\sqrt{3}}, \\quad \\lambda_3 = -\\frac{c}{\\sqrt{3}}\n",
    "$$"
   ]
  },
  {
   "cell_type": "markdown",
   "id": "235de729",
   "metadata": {},
   "source": [
    "To solve for the eigenvectors, we go through each eigenvalue and solve again for the equation $A\\vec{v} = \\lambda\\vec{v}$. For $\\lambda_1 = 0$:\n",
    "$$\n",
    "\\begin{bmatrix} 0 & c^2 n_x & c^2 n_y \\\\ \\frac{1}{3}n_x & 0 & 0 \\\\ \\frac{1}{3}n_y & 0 & 0 \\end{bmatrix} \\begin{bmatrix} v_1 \\\\ v_2 \\\\ v_3 \\end{bmatrix} = \\begin{bmatrix} 0 \\\\ 0 \\\\ 0 \\end{bmatrix}\n",
    "$$\n",
    "From rows 2 and 3, we know immediately that $v_1 = 0$ since each component $n_x$ and $n_y$ are given to be nonzero. The first row gives:\n",
    "$$\n",
    "c^2 n_x v_2 + c^2 n_y v_3 = 0\n",
    "$$\n",
    "So, $v_3 = -\\frac{n_x}{n_y} v_2$. If $v_2 = n_y$:\n",
    "$$\n",
    "\\mathbf{v_1} = \\begin{bmatrix} 0 \\\\ n_y \\\\ -n_x \\end{bmatrix}\n",
    "$$\n",
    "Repeating this process for $\\lambda_2 = \\frac{c}{\\sqrt{3}}$, we once again need to solve the characteristic equation:\n",
    "$$\n",
    "\\begin{bmatrix} 0 - \\frac{c}{\\sqrt{3}} & c^2 n_x & c^2 n_y \\\\ \\frac{1}{3}n_x & 0 - \\frac{c}{\\sqrt{3}} & 0 \\\\ \\frac{1}{3}n_y & 0 & 0 - \\frac{c}{\\sqrt{3}} \\end{bmatrix} \\begin{bmatrix} v_1 \\\\ v_2 \\\\ v_3 \\end{bmatrix} = \\begin{bmatrix} 0 \\\\ 0 \\\\ 0 \\end{bmatrix}\n",
    "$$\n",
    "Equation 1 (row 1):\n",
    "$$-\\frac{c}{\\sqrt{3}}v_1 + c^2 n_x v_2 + c^2 n_y v_3 = 0$$\n",
    "\n",
    "Equation 2 (row 2):\n",
    "$$\\frac{1}{3}n_x v_1 - \\frac{c}{\\sqrt{3}}v_2 = 0$$\n",
    "\n",
    "Equation 3 (row 3):\n",
    "$$\\frac{1}{3}n_y v_1 - \\frac{c}{\\sqrt{3}}v_3 = 0$$\n",
    "\n",
    "We can choose to solve row 2 for $v_2$ and row 3 for $v_3$:\n",
    "$$v_2 = \\frac{n_x v_1}{3} \\left(\\frac{\\sqrt{3}}{c}\\right) = \\frac{\\sqrt{3}n_x v_1}{3c} = \\frac{n_x v_1}{\\sqrt{3}c}$$\n",
    "$$v_3 = \\frac{n_y v_1}{3} \\left(\\frac{\\sqrt{3}}{c}\\right) = \\frac{\\sqrt{3}n_y v_1}{3c} = \\frac{n_y v_1}{\\sqrt{3}c}$$\n",
    "\n",
    "And choosing $v_1 = \\sqrt{3}c$ to eliminate the fractions and simplify:\n",
    "$$v_2 = \\frac{n_x (\\sqrt{3}c)}{\\sqrt{3}c} = n_x$$\n",
    "$$v_3 = \\frac{n_y (\\sqrt{3}c)}{\\sqrt{3}c} = n_y$$\n",
    "\n",
    "We finally get:\n",
    "$$\n",
    "\\mathbf{v_2} = \\begin{bmatrix} \\sqrt{3}c \\\\ n_x \\\\ n_y \\end{bmatrix}\n",
    "$$\n",
    "\n",
    "Repeating the above process for $\\lambda_3 = -\\frac{c}{\\sqrt{3}}$ (and using MATLAB `eig()` to check):\n",
    "$$\n",
    "\\mathbf{v_3} = \\begin{bmatrix} \\sqrt{3}c \\\\ -n_x \\\\ -n_y \\end{bmatrix}\n",
    "$$"
   ]
  },
  {
   "cell_type": "markdown",
   "id": "3510abad",
   "metadata": {},
   "source": [
    "### Part (c)\n",
    "Determine the null space of $\\mathbf{A}$.\n",
    "\n",
    "The null space (kernel) of $\\mathbf{A}$ is all vectors which get transformed to the zero vector after applying $\\mathbf{A}$, i.e. we need to solve:\n",
    "$$\n",
    "\\begin{bmatrix} 0 & c^2 n_x & c^2 n_y \\\\ \\frac{1}{3}n_x & 0 & 0 \\\\ \\frac{1}{3}n_y & 0 & 0 \\end{bmatrix} \\begin{bmatrix} x_1 \\\\ x_2 \\\\ x_3 \\end{bmatrix} = \\begin{bmatrix} 0 \\\\ 0 \\\\ 0 \\end{bmatrix}\n",
    "$$\n",
    "We can notice that this is the same equation we solved for in the $\\lambda_1 = 0$ case, which makes sense. Thus the null space consists of all vectors that satisfy:\n",
    "$$\n",
    "\\mathbf{x} = t \\begin{bmatrix} 0 \\\\ n_y \\\\ -n_x \\end{bmatrix}\n",
    "$$\n",
    "Above, $t$ is any scalar value (any vector that is linearly dependent to $\\mathbf{x}$ is part of the null space)."
   ]
  }
 ],
 "metadata": {
  "language_info": {
   "name": "python"
  }
 },
 "nbformat": 4,
 "nbformat_minor": 5
}
